try out a different way of modeling async writes

src/Hoare.v
@@ -9,10 +9,10 @@ Set Implicit Arguments.
 
 Definition donecond (T: Set) := T -> mem -> Prop.
 
-Definition corr2 (T: Set) (pre: donecond T -> pred -> list mem -> pred) (p: prog T) :=
-  forall done crash m cms out, In m cms
-  -> pre done crash cms m
-  -> exec m cms p out
+Definition corr2 (T: Set) (pre: pred -> donecond T -> pred -> pred) (p: prog T) :=
+  forall precrash done crash m pending out, pre precrash done crash m
+  -> (forall m', apply_some pending m m' -> precrash m')
+  -> exec m pending p out
   -> (exists m' v, out = Finished m' v /\ done v m') \/
      (exists m', out = Crashed T m' /\ crash m').
 
@@ -20,10 +20,11 @@ Notation "{{ pre }} p" := (corr2 pre%pred p)
   (at level 0, p at level 60).
 
 
-Definition corr3 (TF TR: Set) (pre: donecond TF -> donecond TR -> pred)
+Definition corr3 (TF TR: Set) (pre: pred -> donecond TF -> donecond TR -> pred)
                  (p1: prog TF) (p2: prog TR) :=
-  forall done crashdone m out, pre done crashdone m
-  -> exec_recover m p1 p2 out
+  forall precrash done crashdone m pending out, pre precrash done crashdone m
+  -> (forall m', apply_some pending m m' -> precrash m')
+  -> exec_recover m pending p1 p2 out
   -> (exists m' v, out = RFinished TR m' v /\ done v m') \/
      (exists m' v, out = RRecovered TF m' v /\ crashdone v m').
 
@@ -31,26 +32,29 @@ Notation "{{ pre }} p1 >> p2" := (corr3 pre%pred p1 p2)
   (at level 0, p1 at level 60, p2 at level 60).
 
 
-Notation "{< e1 .. e2 , 'PRE' pre 'POST' : r post 'CRASH' crash >} p1" :=
+Notation "{< e1 .. e2 , 'PRE' pre 'PRECRASH' precrash 'POST' : r post 'CRASH' crash >} p1" :=
   (forall T (rx: _ -> prog T), corr2
-   (fun done_ crash_ =>
+   (fun precrash_ done_ crash_ =>
     (exis (fun e1 => .. (exis (fun e2 =>
      exists F,
      F * pre *
+     [[ precrash_ = precrash ]] *
      [[ forall r_,
         {{ fun done'_ crash'_ => (fun r => F * post) r_ * [[ done'_ = done_ ]] * [[ crash'_ = crash_ ]]
-        }} rx r_ ]] * [[ (F * crash)%pred ==> crash_ ]]
+        }} rx r_ ]] *
+     [[ (F * crash)%pred ==> crash_ ]]
      )) .. ))
    )%pred
    (p1 rx)%pred)
   (at level 0, p1 at level 60, e1 binder, e2 binder, r at level 0).
 
-Notation "{< e1 .. e2 , 'PRE' pre 'POST' : rp post 'CRASH' : rc crash 'IDEM' idemcrash >} p1 >> p2" :=
+Notation "{< e1 .. e2 , 'PRE' pre 'PRECRASH' precrash 'POST' : rp post 'CRASH' : rc crash 'IDEM' idemcrash >} p1 >> p2" :=
   (forall TF TR (rxOK: _ -> prog TF) (rxREC: _ -> prog TR), corr3
-   (fun done_ crashdone_ =>
+   (fun precrash_ done_ crashdone_ =>
     (exis (fun e1 => .. (exis (fun e2 =>
      exists F,
      F * pre *
+     [[ precrash_ = precrash ]] *
      [[ forall r_,
         {{ fun done'_ crash'_ => (fun rp => F * post) r_ *
                                  [[ done'_ = done_ ]] * [[ crash'_ ==> F * idemcrash ]]
@@ -69,7 +73,7 @@ Notation "{< e1 .. e2 , 'PRE' pre 'POST' : rp post 'CRASH' : rc crash 'IDEM' ide
 Theorem pimpl_ok2:
   forall T pre pre' (pr: prog T),
   {{pre'}} pr ->
-  (forall done crash cms, pre done crash cms ==> pre' done crash cms) ->
+  (forall precrash done crash, pre precrash done crash ==> pre' precrash done crash) ->
   {{pre}} pr.
 Proof.
   unfold corr2; intros.
@@ -81,7 +85,7 @@ Qed.
 Theorem pimpl_ok3:
   forall TF TR pre pre' (p: prog TF) (r: prog TR),
   {{pre'}} p >> r ->
-  (forall done crashdone, pre done crashdone ==> pre' done crashdone) ->
+  (forall precrash done crashdone, pre precrash done crashdone ==> pre' precrash done crashdone) ->
   {{pre}} p >> r.
 Proof.
   unfold corr3; intros.
@@ -93,35 +97,35 @@ Qed.
 Theorem pimpl_ok2_cont :
   forall T pre pre' A (k : A -> prog T) x y,
   {{pre'}} k y ->
-  (forall done crash cms, pre done crash cms ==> pre' done crash cms) ->
-  (forall done crash cms, pre done crash cms ==> exists F, F * [[x = y]]) ->
+  (forall precrash done crash, pre precrash done crash ==> pre' precrash done crash) ->
+  (forall precrash done crash, pre precrash done crash ==> exists F, F * [[x = y]]) ->
   {{pre}} k x.
 Proof.
   unfold corr2, pimpl; intros.
   edestruct H1; eauto.
   eapply sep_star_lift_l in H5; [|instantiate (1:=([x=y])%pred)].
-  unfold lift in H5; rewrite H5 in *; eauto.
+  unfold lift in *; subst; eauto.
   firstorder.
 Qed.
 
 Theorem pimpl_ok3_cont :
   forall TF TR pre pre' A (k : A -> prog TF) x y (r: prog TR),
   {{pre'}} k y >> r ->
-  (forall done crashdone, pre done crashdone ==> pre' done crashdone) ->
-  (forall done crashdone, pre done crashdone ==> exists F, F * [[x = y]]) ->
+  (forall precrash done crashdone, pre precrash done crashdone ==> pre' precrash done crashdone) ->
+  (forall precrash done crashdone, pre precrash done crashdone ==> exists F, F * [[x = y]]) ->
   {{pre}} k x >> r.
 Proof.
   unfold corr3, pimpl; intros.
   edestruct H1; eauto.
-  eapply sep_star_lift_l in H4; [|instantiate (1:=([x=y])%pred)].
-  unfold lift in H4; rewrite H4 in *; eauto.
+  eapply sep_star_lift_l in H5; [|instantiate (1:=([x=y])%pred)].
+  unfold lift in *; subst; eauto.
   firstorder.
 Qed.
 
 Theorem pimpl_pre2:
   forall T pre pre' (pr: prog T),
-  (forall done crash cms, pre done crash cms ==> [{{pre'}} pr])
-  -> (forall done crash cms, pre done crash cms ==> pre' done crash cms)
+  (forall precrash done crash, pre precrash done crash ==> [{{pre'}} pr])
+  -> (forall precrash done crash, pre precrash done crash ==> pre' precrash done crash)
   -> {{pre}} pr.
 Proof.
   unfold corr2; intros.
@@ -132,8 +136,8 @@ Qed.
 
 Theorem pimpl_pre3:
   forall TF TR pre pre' (p: prog TF) (r: prog TR),
-  (forall done crashdone, pre done crashdone ==> [{{pre'}} p >> r])
-  -> (forall done crashdone, pre done crashdone ==> pre' done crashdone)
+  (forall precrash done crashdone, pre precrash done crashdone ==> [{{pre'}} p >> r])
+  -> (forall precrash done crashdone, pre precrash done crashdone ==> pre' precrash done crashdone)
   -> {{pre}} p >> r.
 Proof.
   unfold corr3; intros.
@@ -142,28 +146,28 @@ Proof.
   eauto.
 Qed.
 
-(*
 Theorem pre_false2:
   forall T pre (p: prog T),
-  (forall done crash, pre done crash ==> [False])
+  (forall precrash done crash, pre precrash done crash ==> [False])
   -> {{ pre }} p.
 Proof.
-  firstorder.
+  unfold corr2; intros; exfalso.
+  eapply H; eauto.
 Qed.
 
 Theorem pre_false3:
   forall TF TR pre (p: prog TF) (r: prog TR),
-  (forall done crashdone, pre done crashdone ==> [False])
+  (forall precrash done crashdone, pre precrash done crashdone ==> [False])
   -> {{ pre }} p >> r.
 Proof.
-  firstorder.
+  unfold corr3; intros; exfalso.
+  eapply H; eauto.
 Qed.
-
 
 Theorem corr2_exists:
   forall T R pre (p: prog R),
-  (forall (a:T), {{ fun done crash => pre done crash a }} p)
-  -> {{ fun done crash => exists a:T, pre done crash a }} p.
+  (forall (a:T), {{ fun precrash done crash => pre precrash done crash a }} p)
+  -> {{ fun precrash done crash => exists a:T, pre precrash done crash a }} p.
 Proof.
   unfold corr2; intros.
   destruct H0.
@@ -172,8 +176,8 @@ Qed.
 
 Theorem corr3_exists:
   forall T RF RR pre (p: prog RF) (r: prog RR),
-  (forall (a:T), {{ fun done crashdone => pre done crashdone a }} p >> r)
-  -> {{ fun done crashdone => exists a:T, pre done crashdone a }} p >> r.
+  (forall (a:T), {{ fun precrash done crashdone => pre precrash done crashdone a }} p >> r)
+  -> {{ fun precrash done crashdone => exists a:T, pre precrash done crashdone a }} p >> r.
 Proof.
   unfold corr3; intros.
   destruct H0.
@@ -181,22 +185,19 @@ Proof.
 Qed.
 
 Theorem corr2_forall: forall T R pre (p: prog R),
-  {{ fun done crash => exists a:T, pre done crash a }} p
-  -> forall (a:T), {{ fun done crash => pre done crash a }} p.
+  {{ fun precrash done crash => exists a:T, pre precrash done crash a }} p
+  -> forall (a:T), {{ fun precrash done crash => pre precrash done crash a }} p.
 Proof.
   unfold corr2; intros.
-  eapply H.
+  eapply H; eauto.
   exists a; eauto.
-  eauto.
 Qed.
 
 Theorem corr3_forall: forall T RF RR pre (p: prog RF) (r: prog RR),
-  {{ fun done crashdone => exists a:T, pre done crashdone a }} p >> r
-  -> forall (a:T), {{ fun done crashdone => pre done crashdone a }} p >> r.
+  {{ fun precrash done crashdone => exists a:T, pre precrash done crashdone a }} p >> r
+  -> forall (a:T), {{ fun precrash done crashdone => pre precrash done crashdone a }} p >> r.
 Proof.
   unfold corr3; intros.
-  eapply H.
+  eapply H; eauto.
   exists a; eauto.
-  eauto.
 Qed.
-*)
